Begin refinement proof.

rif/abstract.v
@@ -14,6 +14,8 @@ Variable Σ : finType.
 Variable mt : machine_types.
 Variable mops : machine_ops mt.
 Variable r_arg : reg mt.
+Variable output_addr : mword mt.
+Variable reclassify_addr : mword mt.
 
 Local Notation rifAutomaton := (rifAutomaton Σ).
 Local Notation rifLabel := (rifLabel Σ).
@@ -29,14 +31,11 @@ Inductive ainstr : Type :=
 | AStore of reg mt & reg mt
 | AJump of reg mt
 | ABnz of reg mt & imm mt
-| AJal of reg mt & Σ
-| AHalt
-| AOutput
-| AReclassify.
+| AJal of reg mt & option Σ
+| AHalt.
 
 Record state := State {
-  imem    : {partmap mword mt -> ainstr};
-  dmem    : {partmap mword mt -> atom};
+  mem     : {partmap mword mt -> ainstr + atom};
   regs    : {partmap reg mt -> atom};
   pc      : atom;
   reclass : option Σ
@@ -48,64 +47,82 @@ Local Open Scope rif_scope.
 Implicit Type s : state.
 
 Definition step s : option (state * option event) :=
-  let: State imem dmem regs pc@lpc reclass := s in
-  do! i <- imem pc;
-  match i with
-  | ANop => Some (State imem dmem regs (pc + 1)@lpc None, None)
-  | AConst k r =>
-    do! regs <- updm regs r (swcast k)@⊥ₗ;
-    Some (State imem dmem regs (pc + 1)@lpc None, None)
-  | AMov r1 r2 =>
-    do! v <- regs r1;
-    do! regs <- updm regs r2 v;
-    Some (State imem dmem regs (pc + 1)@lpc None, None)
-  | ABinop o r1 r2 r3 =>
-    do! v1 <- regs r1;
-    do! v2 <- regs r2;
-    do! regs <- updm regs r3 (binop_denote o (vala v1) (vala v2))@(taga v1 ⊔ₗ taga v2);
-    Some (State imem dmem regs (pc + 1)@lpc None, None)
-  | ALoad r1 r2 =>
-    do! v1 <- regs r1;
-    do! v2 <- dmem (vala v1);
-    do! regs <- updm regs r2 (vala v2)@(taga v1 ⊔ₗ taga v2);
-    Some (State imem dmem regs (pc + 1)@lpc None, None)
-  | AStore r1 r2 =>
-    do! v1 <- regs r1;
-    do! v2 <- regs r2;
-    do! vold <- dmem (vala v1);
-    if taga v1 ⊔ₗ lpc ⊑ₗ taga vold then
-      do! dmem <- updm dmem (vala v1)
-                            (vala v2)@(taga v1 ⊔ₗ taga v2 ⊔ₗ lpc);
-      Some (State imem dmem regs (pc + 1)@lpc None, None)
+  let: State mem regs pc@lpc reclass := s in
+  if mem pc is Some i then
+    if i is inl i then
+      match i with
+      | ANop => Some (State mem regs (pc + 1)@lpc None, None)
+      | AConst k r =>
+        do! regs <- updm regs r (swcast k)@⊥ₗ;
+        Some (State mem regs (pc + 1)@lpc None, None)
+      | AMov r1 r2 =>
+        do! v <- regs r1;
+        do! regs <- updm regs r2 v;
+        Some (State mem regs (pc + 1)@lpc None, None)
+      | ABinop o r1 r2 r3 =>
+        do! v1 <- regs r1;
+        do! v2 <- regs r2;
+        do! regs <- updm regs r3 (binop_denote o (vala v1) (vala v2))@(taga v1 ⊔ₗ taga v2);
+        Some (State mem regs (pc + 1)@lpc None, None)
+      | ALoad r1 r2 =>
+        do! v1 <- regs r1;
+        do! v2 <- mem (vala v1);
+        if v2 is inr v2 then
+          do! regs <- updm regs r2 (vala v2)@(taga v1 ⊔ₗ taga v2);
+          Some (State mem regs (pc + 1)@lpc None, None)
+        else None
+      | AStore r1 r2 =>
+        do! v1 <- regs r1;
+        do! v2 <- regs r2;
+        do! vold <- mem (vala v1);
+        if vold is inr vold then
+          if taga v1 ⊔ₗ lpc ⊑ₗ taga vold then
+            do! mem <- updm mem (vala v1)
+                                (inr (vala v2)@(taga v1 ⊔ₗ taga v2 ⊔ₗ lpc));
+            Some (State mem regs (pc + 1)@lpc None, None)
+          else None
+        else None
+      | AJump r =>
+        do! v <- regs r;
+        Some (State mem regs (vala v)@(taga v ⊔ₗ lpc) None, None)
+      | ABnz r x =>
+        do! v <- regs r;
+        let pc' := pc + if vala v == 0 then 1
+                        else swcast x in
+        Some (State mem regs pc'@(taga v ⊔ₗ lpc) None, None)
+      | AJal r oF =>
+        do! v <- regs r;
+        do! regs <- updm regs ra (pc + 1)@(taga v ⊔ₗ lpc);
+        Some (State mem regs (vala v)@(taga v ⊔ₗ lpc) oF, None)
+      | AHalt => None
+      end
     else None
-  | AJump r =>
-    do! v <- regs r;
-    Some (State imem dmem regs (vala v)@(taga v ⊔ₗ lpc) None, None)
-  | ABnz r x =>
-    do! v <- regs r;
-    let pc' := pc + if vala v == 0 then 1
-                    else swcast x in
-    Some (State imem dmem regs pc'@(taga v ⊔ₗ lpc) None, None)
-  | AJal r F =>
-    do! v <- regs r;
-    do! regs <- updm regs ra (pc + 1)@(taga v ⊔ₗ lpc);
-    Some (State imem dmem regs (vala v)@(taga v ⊔ₗ lpc) (Some F), None)
-  | AHalt => None
-  | AOutput =>
+  else if pc == output_addr then
     do! raddr <- regs ra;
     do! out   <- regs r_arg;
     let r_pc  := rif_readers _ (rif_state (taga raddr)) in
     let r_out := rif_readers _ (rif_state (taga out)) in
-    Some (State imem dmem regs raddr None,
+    Some (State mem regs raddr None,
           Some (Output _ (vala out) (r_pc ⊔ᵣ r_out)))
-  | AReclassify =>
+  else if pc == reclassify_addr then
     do! raddr <- regs ra;
     do! arg   <- regs r_arg;
     if reclass is Some F then
       do! regs  <- updm regs r_arg (vala arg)@(rl_trans (taga arg) F);
-      Some (State imem dmem regs raddr None,
+      Some (State mem regs raddr None,
             Some (Reclassify _ (taga arg) F))
     else None
-  end.
+  else None.
 
 End Abstract.
+
+Arguments ANop {Σ mt}.
+Arguments AConst {Σ mt} _ _.
+Arguments AMov {Σ mt} _ _.
+Arguments ABinop {Σ mt} _ _ _ _.
+Arguments ALoad {Σ mt} _ _.
+Arguments AStore {Σ mt} _ _.
+Arguments AJump {Σ mt} _.
+Arguments ABnz {Σ mt} _ _.
+Arguments AJal {Σ mt} _ _.
+Arguments AHalt {Σ mt}.
