rif/refinementSA.v
@@ -1,0 +1,172 @@
+From mathcomp Require Import ssreflect ssrfun ssrbool ssrnat eqtype seq fintype finfun.
+From CoqUtils Require Import hseq ord fset partmap word.
+From MicroPolicies Require Import
+  lib.utils lib.partmap_utils common.types symbolic.symbolic symbolic.exec
+  rif.common rif.symbolic rif.abstract.
+
+Set Implicit Arguments.
+Unset Strict Implicit.
+Unset Printing Implicit Defensive.
+
+Section Abstract.
+
+Import DoNotation.
+
+Variable Σ : finType.
+Variable mt : machine_types.
+Variable mops : machine_ops mt.
+Variable r_arg : reg mt.
+
+Local Notation rifAutomaton := (rifAutomaton Σ).
+Local Notation rifLabel := (rifLabel Σ).
+Local Notation event := (event Σ mt).
+Local Notation word := (mword mt).
+Local Notation d_atom := (atom word rifLabel).
+
+Variable output_addr : word.
+Variable reclassify_addr : word.
+
+Local Notation sstate := (@Symbolic.state mt (sym_rif Σ mt)).
+Local Notation sstep :=
+  (@stepf _ _ _ (@rif_syscalls Σ mt mops output_addr reclassify_addr r_arg)).
+Local Notation astate := (rif.abstract.state Σ mt).
+Local Notation astep := (@step Σ mt mops r_arg output_addr reclassify_addr).
+Local Notation ainstr := (ainstr Σ mt).
+
+Implicit Types (sst : sstate) (ast : astate).
+
+Local Open Scope rif_scope.
+
+Definition abs_instr (i : word) (oF : option Σ) : option ainstr :=
+  if decode_instr i is Some i then
+    match i with
+    | Nop => Some ANop
+    | Const i r => Some (AConst i r)
+    | Mov r1 r2 => Some (AMov r1 r2)
+    | Binop o r1 r2 r3 => Some (ABinop o r1 r2 r3)
+    | Load r1 r2 => Some (ALoad r1 r2)
+    | Store r1 r2 => Some (AStore r1 r2)
+    | Jump r => Some (AJump r)
+    | Bnz r i => Some (ABnz r i)
+    | Jal r => Some (AJal r oF)
+    | Halt => Some AHalt
+    | JumpEpc | AddRule  | GetTag _ _  | PutTag _ _ _ => None
+    end
+  else None.
+
+Definition refine_m_atom (x : atom word (mem_tag Σ)) (y : ainstr + d_atom) :=
+  match x, y with
+  | wx@(MemInstr oF), inl i => abs_instr wx oF = Some i
+  | wx@(MemData rl), inr a => wx@rl = a
+  | _, _ => False
+  end.
+
+Inductive refine_state sst ast : Prop :=
+| RefineState of pointwise refine_m_atom (Symbolic.mem sst) (rif.abstract.mem ast)
+              &  Symbolic.regs sst = rif.abstract.regs ast
+              &  vala (Symbolic.pc sst) = vala (rif.abstract.pc ast)
+              &  (taga (Symbolic.pc sst)).1 = taga (rif.abstract.pc ast)
+              &  (taga (Symbolic.pc sst)).2 = rif.abstract.reclass ast.
+
+Hint Unfold Symbolic.next_state_pc.
+Hint Unfold Symbolic.next_state_reg.
+Hint Unfold Symbolic.next_state_reg_and_pc.
+Hint Unfold Symbolic.next_state.
+
+Lemma refinement sst sst' ast :
+  refine_state sst ast ->
+  sstep sst = Some sst' ->
+  match astep ast with
+  | Some (ast', oe) =>
+    refine_state sst' ast'
+    /\ Symbolic.internal sst' =
+       Symbolic.internal sst ++ oapp (cons ^~ [::]) [::] oe
+  | None => False
+  end.
+Proof.
+rewrite (lock sstep) (lock astep).
+case: sst=> /= sm sr [spc [slpc src]] t.
+case: ast=> /= am ar [apc alpc] arc.
+case=> /= ref_m ref_r.
+move: sr ref_r=> regs <- {ar}.
+move: spc slpc src => pc lpc rc <- <- <- {apc alpc arc}.
+rewrite -lock /=.
+move: (ref_m pc).
+case: (sm pc) => [[si [oF|sti]]|]; case aget_pc: (am pc) => [[ai|?]|] //=.
+- (* Instruction *)
+  rewrite /abs_instr.
+  case: decode_instr => [i|] ref_i //=.
+  case: i ref_i aget_pc => //=; repeat autounfold=> /=.
+  + (* Nop *)
+    move=> [<-] {ai} aget_pc [<-] {sst'}.
+    by rewrite -lock /= aget_pc /= cats0; split.
+  + (* Const *)
+    move=> i r [<-] {ai} aget_pc.
+    case: (regs r)=> //= - [_ _].
+    case upd_r: updm => [regs'|] //= [<-] {sst'}.
+    by rewrite -lock /= aget_pc /= upd_r /= cats0; split.
+  + (* Mov *)
+    move=> r1 r2 [<-] {ai} aget_pc.
+    case get_r1: (regs r1)=> [[w1 rl1]|] //=.
+    case: (regs r2)=> //= - [_ _].
+    case upd_r2: updm => [regs'|] //= [<-] {sst'}.
+    by rewrite -lock /= aget_pc get_r1 /= upd_r2 /= cats0; split.
+  + (* Binop *)
+    move=> b r1 r2 r3 [<-] {ai} aget_pc.
+    case get_r1: (regs r1)=> [[w1 rl1]|] //=.
+    case get_r2: (regs r2)=> [[w2 rl2]|] //=.
+    case: (regs r3)=> [[_ _]|] //=.
+    case upd_r3: updm=> [regs'|] //= [<-] {sst'}.
+    by rewrite -lock /= aget_pc get_r1 /= get_r2 /= upd_r3 /= cats0; split.
+  + (* Load *)
+    move=> r1 r2 [<-] {ai} aget_pc.
+    case get_r1: (regs r1)=> [[w1 rl1]|] //=.
+    move: (ref_m w1).
+    case sget_w1: (sm w1) => [[w1' [oF'|rl1']]|] //=;
+    case: (regs r2)=> [[_ _]|] //=.
+    case aget_w1: (am w1) => [[?|a]|] //= e.
+    move: e aget_w1=> <- {a} aget_w1.
+    case upd_r2: updm => [regs'|] //= [<-] {sst'}.
+    by rewrite -lock /= aget_pc get_r1 /= aget_w1 /= upd_r2 /= cats0; split.
+  + (* Store *)
+    move=> r1 r2 [<-] {ai} aget_pc.
+    case get_r1: (regs r1)=> [[w1 rl1]|] //=.
+    case sget_w1: (sm w1) => [[wold [oF'|rlold]]|] //=;
+    case get_r2: (regs r2)=> [[w2 rl2]|] //=.
+    case: ifP => // check /=.
+    case supd_w1: updm => [sm'|] //= [<-] {sst'}.
+    have [am' aupd_w1]:
+      exists am', updm am w1 (inr w2@(rl1 ⊔ₗ rl2 ⊔ₗ lpc)) = Some am'.
+      exists (setm am w1 (inr w2@(rl1 ⊔ₗ rl2 ⊔ₗ lpc))).
+      move: (ref_m w1) supd_w1; rewrite /updm.
+      by case: (sm w1) (am w1) => //= sa [aa|] //= {sa aa} _ [<-].
+    have ref_a: refine_m_atom w2@(MemData (rl1 ⊔ₗ rl2 ⊔ₗ lpc))
+                              (inr w2@(rl1 ⊔ₗ rl2 ⊔ₗ lpc)) by [].
+    have ref_m' := refine_upd_pointwise2 ref_m ref_a supd_w1 aupd_w1.
+    move: (ref_m w1); rewrite sget_w1 /=.
+    case aget_w1: (am w1) => [[?|a]|] //= e.
+    move: e aget_w1 => <- {a} aget_w1.
+    rewrite -lock /= aget_pc get_r1 /= get_r2 /= aget_w1 /= check aupd_w1 /=.
+    by rewrite cats0; split.
+  + (* Jump *)
+    move=> r [<-] {ai} aget_pc.
+    case get_r: (regs r)=> [[w1 rl1]|] //= [<-] {sst'}.
+    by rewrite -lock /= aget_pc get_r /= cats0; split.
+  + (* Bnz *)
+    move=> r i [<-] {ai} aget_pc.
+    case get_r: (regs r)=> [[w1 rl1]|] //= [<-] {sst'}.
+    by rewrite -lock /= aget_pc get_r /= cats0; split.
+  (* Jal *)
+  move=> r [<-] {ai} aget_pc.
+  case get_r: (regs r) => [[w1 rl1]|] //=.
+  case: (regs ra)=> [[_ _]|] //=.
+  case upd_ra: updm => [regs'|] //= [<-] {sst'}.
+  by rewrite -lock /= aget_pc /= get_r /= upd_ra /= cats0; split.
+- (* Fetch data in memory instead of instruction; contradiction *)
+  admit.
+(* System service *)
+move=> _ /=.
+admit.
+Admitted.
+
+End Abstract.
